michael_formal/drinks_machine2.thy
@@ -2,41 +2,41 @@ theory drinks_machine2
   imports drinks_machine Contexts
 begin
 
-abbreviation vend2 :: "efsm" where
+abbreviation drinks2 :: "efsm" where
 (* Effectively this is the drinks_machine which has had the loop unrolled by one iteration *)
-"vend2 \<equiv> \<lparr> S = [1,2,3,4],
+"drinks2 \<equiv> \<lparr> S = [1,2,3,4],
           s0 = 1,
           T = \<lambda> (a,b) . 
-              if (a,b) = (1,2) then [t1]
-              else if (a,b) = (2,3) then [t2]
-              else if (a,b) = (3,3) then [t2]
-              else if (a,b) = (3,4) then [t3]
+              if (a,b) = (1,2) then [select]
+              else if (a,b) = (2,3) then [coin]
+              else if (a,b) = (3,3) then [coin]
+              else if (a,b) = (3,4) then [vend]
               else []
          \<rparr>"
 
-lemma "observe_trace vend2 (s0 vend2) <> [] = []"
+lemma "observe_trace drinks2 (s0 drinks2) <> [] = []"
   by simp
 
-lemma "observe_trace vend2 (s0 vend2) <> [(''select'', [Str ''coke''])] = [[]]"
-  by (simp add: step_def t1_def)
+lemma "observe_trace drinks2 (s0 drinks2) <> [(''select'', [Str ''coke''])] = [[]]"
+  by (simp add: step_def select_def)
 
-lemma "observe_trace vend2 (s0 vend2) <> [(''select'', [Str ''coke'']), (''coin'', [Num 50])] = [[], [Num 50]]"
-  by (simp add: step_def t1_def t2_def)
+lemma "observe_trace drinks2 (s0 drinks2) <> [(''select'', [Str ''coke'']), (''coin'', [Num 50])] = [[], [Num 50]]"
+  by (simp add: step_def select_def coin_def)
 
-lemma "observe_trace vend2 (s0 vend2) <> [(''select'', [Str ''coke'']), (''coin'', [Num 50]), (''coin'', [Num 50])] = [[], [Num 50], [Num 100]]"
+lemma "observe_trace drinks2 (s0 drinks2) <> [(''select'', [Str ''coke'']), (''coin'', [Num 50]), (''coin'', [Num 50])] = [[], [Num 50], [Num 100]]"
   by (simp add: step_def transitions)
 
-lemma "observe_trace vend2 (s0 vend2) <> [(''select'', [Str ''coke'']), (''coin'', [Num 50]), (''coin'', [Num 50]), (''vend'', [])] = [[], [Num 50], [Num 100], [Str ''coke'']]"
+lemma "observe_trace drinks2 (s0 drinks2) <> [(''select'', [Str ''coke'']), (''coin'', [Num 50]), (''coin'', [Num 50]), (''vend'', [])] = [[], [Num 50], [Num 100], [Str ''coke'']]"
   by (simp add: step_def transitions)
 
-lemma "equiv vend vend2 [(''select'', [Str ''coke'']), (''coin'', [Num 50]), (''coin'', [Num 50]), (''vend'', [])]"
-  by (simp add: equiv_def step_def vend_def transitions)
+lemma "equiv drinks drinks2 [(''select'', [Str ''coke'']), (''coin'', [Num 50]), (''coin'', [Num 50]), (''vend'', [])]"
+  by (simp add: equiv_def step_def drinks_def transitions)
 
-abbreviation t1_posterior :: "context" where
-  "t1_posterior \<equiv> \<lbrakk>(V (R 1)) \<mapsto> Bc True, (V (R 2)) \<mapsto> Eq (Num 0) \<rbrakk>"
+abbreviation select_posterior :: "context" where
+  "select_posterior \<equiv> \<lbrakk>(V (R 1)) \<mapsto> Bc True, (V (R 2)) \<mapsto> Eq (Num 0) \<rbrakk>"
 
-lemma "consistent (medial empty (Guard t1))"
-  by (simp add: t1_def)
+lemma "consistent (medial empty (Guard select))"
+  by (simp add: select_def)
 
 lemma empty_not_undef: "empty r \<noteq> Undef \<longrightarrow> empty r = Bc True"
   apply (insert consistent_empty_1)
@@ -51,27 +51,27 @@ lemma empty_never_false: "cexp.Bc False \<noteq> Contexts.empty x"
 lemma foo: "\<not> (x \<noteq> V (R 1) \<and> x \<noteq> V (R 2) \<and> (x = V (R 1) \<or> x = V (R 2)))"
   by auto
 
-lemma consistent_medial_t2: "consistent \<lbrakk>V (R 1) \<mapsto> cexp.Bc True, V (R 2) \<mapsto> cexp.Eq (Num 0)\<rbrakk>"
+lemma consistent_medial_coin: "consistent \<lbrakk>V (R 1) \<mapsto> cexp.Bc True, V (R 2) \<mapsto> cexp.Eq (Num 0)\<rbrakk>"
   apply (simp add: consistent_def)
   apply (rule_tac x="<R 1 := Num 0, R 2 := Num 0>" in exI)
   apply (simp del: Nat.One_nat_def)
   using consistent_empty_4 by auto
 
-lemma posterior_t2_first: "posterior t1_posterior t2 = \<lbrakk>(V (R 1)) \<mapsto> Bc True, (V (R 2)) \<mapsto> Bc True\<rbrakk>"
-  apply (simp add: posterior_def consistent_medial_t2 del: Nat.One_nat_def)
-  apply (simp add: t2_def valid_def satisfiable_def)
+lemma posterior_coin_first: "posterior select_posterior coin = \<lbrakk>(V (R 1)) \<mapsto> Bc True, (V (R 2)) \<mapsto> Bc True\<rbrakk>"
+  apply (simp add: posterior_def consistent_medial_coin del: Nat.One_nat_def)
+  apply (simp add: coin_def valid_def satisfiable_def)
   apply (rule ext)
   by simp
 
-lemma consistent_medial_t2_2: "consistent \<lbrakk>V (R (Suc 0)) \<mapsto> cexp.Bc True, V (R 2) \<mapsto> cexp.Bc True\<rbrakk>"
+lemma consistent_medial_coin_2: "consistent \<lbrakk>V (R (Suc 0)) \<mapsto> cexp.Bc True, V (R 2) \<mapsto> cexp.Bc True\<rbrakk>"
   apply (simp add: consistent_def)
   apply (rule_tac x="<>" in exI)
   apply (simp del: Nat.One_nat_def)
   using consistent_empty_4 by auto
 
-lemma posterior_t2_subsequent: "posterior \<lbrakk>V (R (Suc 0)) \<mapsto> cexp.Bc True, V (R 2) \<mapsto> cexp.Bc True\<rbrakk> t2 = \<lbrakk>V (R (Suc 0)) \<mapsto> cexp.Bc True, V (R 2) \<mapsto> cexp.Bc True\<rbrakk>"
-  apply (simp add: posterior_def consistent_medial_t2_2)
-  apply (simp add: t2_def valid_def satisfiable_def)
+lemma posterior_coin_subsequent: "posterior \<lbrakk>V (R (Suc 0)) \<mapsto> cexp.Bc True, V (R 2) \<mapsto> cexp.Bc True\<rbrakk> coin = \<lbrakk>V (R (Suc 0)) \<mapsto> cexp.Bc True, V (R 2) \<mapsto> cexp.Bc True\<rbrakk>"
+  apply (simp add: posterior_def consistent_medial_coin_2)
+  apply (simp add: coin_def valid_def satisfiable_def)
   apply (rule ext)
   by simp
 
@@ -117,9 +117,9 @@ lemma "context_equiv (Contexts.apply_guard \<lbrakk>(V (R 1)) \<mapsto> Bc True\
   apply (case_tac r)
   by simp_all
 
-(* You can't take t3 immediately after taking t1 *)
-lemma r2_0_t3: "\<not>Contexts.can_take t3 t1_posterior"
-  apply (simp only: t3_def Contexts.can_take_def)
+(* You can't take vend immediately after taking select *)
+lemma r2_0_vend: "\<not>Contexts.can_take vend select_posterior"
+  apply (simp only: vend_def Contexts.can_take_def)
   apply (simp only: consistent_def)
   apply (simp del: Nat.One_nat_def)
   apply (rule allI)
@@ -133,7 +133,7 @@ lemma r2_0_t3: "\<not>Contexts.can_take t3 t1_posterior"
   apply (simp del: Nat.One_nat_def)
   by fastforce
 
-lemma consistent_t1_posterior: "consistent t1_posterior"
+lemma consistent_select_posterior: "consistent select_posterior"
   apply (simp add: consistent_def)
   apply (rule_tac x="<R 1 := Num 0, R 2 := Num 0>" in exI)
   apply (simp del: Nat.One_nat_def)
@@ -146,8 +146,8 @@ lemma consistent_t1_posterior: "consistent t1_posterior"
 lemma can_take_no_guards: "\<forall> c. (Contexts.consistent c \<and> (Guard t) = []) \<longrightarrow> Contexts.can_take t c"
   by (simp add: consistent_def Contexts.can_take_def)
 
-lemma can_take_t2: "consistent c \<longrightarrow> Contexts.can_take t2 c"
-  by (simp add: t2_def consistent_def Contexts.can_take_def)
+lemma can_take_coin: "consistent c \<longrightarrow> Contexts.can_take coin c"
+  by (simp add: coin_def consistent_def Contexts.can_take_def)
 
 abbreviation r1_r2_true :: "context" where
 "r1_r2_true \<equiv> \<lbrakk>(V (R 1)) \<mapsto> Bc True, (V (R 2)) \<mapsto> Bc True\<rbrakk>"
@@ -158,42 +158,42 @@ lemma consistent_r1_r2_true: "consistent r1_r2_true"
   apply (simp del: Nat.One_nat_def)
   using consistent_empty_1 by force
 
-lemma t1_posterior: "(posterior empty t1) = t1_posterior"
-  apply (simp add: posterior_def t1_def)
+lemma select_posterior: "(posterior empty select) = select_posterior"
+  apply (simp add: posterior_def select_def)
   apply (rule ext)
   by simp
 
-lemma posterior_r1_r2_true_t2: "(posterior r1_r2_true t2) = r1_r2_true"
-  apply (simp add: posterior_def t2_def consistent_def satisfiable_def valid_def)
+lemma posterior_r1_r2_true_coin: "(posterior r1_r2_true coin) = r1_r2_true"
+  apply (simp add: posterior_def coin_def consistent_def satisfiable_def valid_def)
   apply safe
    apply auto[1]
   using consistent_empty_1 by force
 
-lemma t2_empty: "(posterior r1_r2_true t2) = r1_r2_true"
+lemma coin_empty: "(posterior r1_r2_true coin) = r1_r2_true"
   apply (rule ext)
-  apply (simp add: posterior_def t2_def satisfiable_def consistent_def)
+  apply (simp add: posterior_def coin_def satisfiable_def consistent_def)
   using empty_not_undef by force
 
-lemma valid_t2_empty: "valid_context (posterior r1_r2_true t2)"
-  apply (simp add: posterior_r1_r2_true_t2)
+lemma valid_coin_empty: "valid_context (posterior r1_r2_true coin)"
+  apply (simp add: posterior_r1_r2_true_coin)
   apply (simp add: valid_context_def)
-  apply (simp add: posterior_t2_subsequent)
+  apply (simp add: posterior_coin_subsequent)
   by (simp add: consistent_empty_4)
 
 lemma valid_true: "valid c \<longrightarrow> cexp_equiv c (Bc True)"
   apply (simp add: valid_def cexp_equiv_def)
   by auto
 
-lemma consistent_medial_t2_3: "consistent (\<lambda>a. if a = V (R 2) then cexp.Eq (Num 0) else if a = V (R 1) then cexp.Bc True else \<lbrakk>\<rbrakk> a)"
+lemma consistent_medial_coin_3: "consistent (\<lambda>a. if a = V (R 2) then cexp.Eq (Num 0) else if a = V (R 1) then cexp.Bc True else \<lbrakk>\<rbrakk> a)"
   apply (simp add: consistent_def)
   apply (rule_tac x="<R 1 := Num 0, R 2 := Num 0>" in exI)
   apply (simp del: Nat.One_nat_def)
   by (simp add: consistent_empty_4)
 
-lemma posterior_t2_true: "(posterior (\<lambda>a. if a = V (R 2) then cexp.Eq (Num 0) else if a = V (R 1) then cexp.Bc True else \<lbrakk>\<rbrakk> a) t2) = r1_r2_true"
+lemma posterior_coin_true: "(posterior (\<lambda>a. if a = V (R 2) then cexp.Eq (Num 0) else if a = V (R 1) then cexp.Bc True else \<lbrakk>\<rbrakk> a) coin) = r1_r2_true"
   apply (simp add: posterior_def)
-  apply (simp add: consistent_medial_t2_3)
-  apply (simp add: t2_def valid_def satisfiable_def)
+  apply (simp add: consistent_medial_coin_3)
+  apply (simp add: coin_def valid_def satisfiable_def)
   apply (rule ext)
   by simp
 
@@ -201,26 +201,26 @@ lemma r1_r2_true_equiv: "(\<lambda>a. if a = V (R 2) then cexp.Bc True else if a
   apply (rule ext)
   by simp
 
-lemma posterior_t2_true_true: "posterior r1_r2_true t2 = r1_r2_true"
-  using posterior_r1_r2_true_t2 by blast
+lemma posterior_coin_true_true: "posterior r1_r2_true coin = r1_r2_true"
+  using posterior_r1_r2_true_coin by blast
 
-lemma r2_0_r1_true_equiv: "(\<lambda>a. if a = V (R 2) then cexp.Eq (Num 0) else if a = V (R 1) then cexp.Bc True else \<lbrakk>\<rbrakk> a) = t1_posterior"
+lemma r2_0_r1_true_equiv: "(\<lambda>a. if a = V (R 2) then cexp.Eq (Num 0) else if a = V (R 1) then cexp.Bc True else \<lbrakk>\<rbrakk> a) = select_posterior"
   apply (rule ext)
   by simp
 
-lemma posterior_n_t2_true_true: "(posterior_n n t2 r1_r2_true) = r1_r2_true"
+lemma posterior_n_coin_true_true: "(posterior_n n coin r1_r2_true) = r1_r2_true"
 proof (induct n)
   case 0
   then show ?case by simp
 next
   case (Suc n)
   then show ?case
-    apply (simp add: r1_r2_true_equiv posterior_t2_subsequent  del: Nat.One_nat_def)
-    by (simp only: posterior_t2_true_true)
+    apply (simp add: r1_r2_true_equiv posterior_coin_subsequent  del: Nat.One_nat_def)
+    by (simp only: posterior_coin_true_true)
 qed
 
-(* We can go round t2 as many times as we like *)
-lemma consistent_posterior_n_t2: "consistent (posterior_n n t2 t1_posterior)"
+(* We can go round coin as many times as we like *)
+lemma consistent_posterior_n_coin: "consistent (posterior_n n coin select_posterior)"
 proof(induct n)
   case 0
   then show ?case 
@@ -233,54 +233,54 @@ next
   then show ?case
     apply (simp del: Nat.One_nat_def)
     apply (simp add: r2_0_r1_true_equiv del: Nat.One_nat_def)
-    apply (simp only:  posterior_t2_first posterior_n_t2_true_true)
+    apply (simp only:  posterior_coin_first posterior_n_coin_true_true)
     using consistent_r1_r2_true by blast
 qed
 
 (* We have to do a "coin" before we can do a "vend"*)
-lemma coin_before_vend: "Contexts.can_take t3 (posterior_n n t2 (posterior \<lbrakk>\<rbrakk> t1)) \<longrightarrow> n > 0"
-  apply (simp add: t1_posterior del: Nat.One_nat_def)
+lemma coin_before_vend: "Contexts.can_take vend (posterior_n n coin (posterior \<lbrakk>\<rbrakk> select)) \<longrightarrow> n > 0"
+  apply (simp add: select_posterior del: Nat.One_nat_def)
   apply (cases n)
-   apply (simp add: r2_0_t3 del: Nat.One_nat_def)
+   apply (simp add: r2_0_vend del: Nat.One_nat_def)
   by simp
 
-lemma posterior_n_t2_true_2: "(posterior_n (Suc n) t2 t1_posterior) = r1_r2_true"
+lemma posterior_n_coin_true_2: "(posterior_n (Suc n) coin select_posterior) = r1_r2_true"
 proof (induct n)
   case 0
   then show ?case
     apply (simp del: Nat.One_nat_def)
-    apply (simp only: r2_0_r1_true_equiv posterior_t2_first)
+    apply (simp only: r2_0_r1_true_equiv posterior_coin_first)
     apply (rule ext)
     by simp
 next
   case (Suc n)
   then show ?case
     apply (simp del: Nat.One_nat_def)
-    apply (simp only: r2_0_r1_true_equiv posterior_t2_first)
+    apply (simp only: r2_0_r1_true_equiv posterior_coin_first)
     apply (simp only: r1_r2_true_equiv)
-    apply (simp add: posterior_t2_subsequent)
+    apply (simp add: posterior_coin_subsequent)
     apply (rule ext)
     by simp
 qed
 
-lemma can_take_t3: "0 < Suc n \<longrightarrow> Contexts.can_take t3 r1_r2_true"
-  apply (simp add: can_take_def consistent_def t3_def)
+lemma can_take_vend: "0 < Suc n \<longrightarrow> Contexts.can_take vend r1_r2_true"
+  apply (simp add: can_take_def consistent_def vend_def)
   apply (rule_tac x="<R 1 := Num 0, R 2 := Num 100>" in exI)
   by (simp add: consistent_empty_4)
 
-lemma medial_t3: "medial r1_r2_true (Guard t3) = \<lbrakk>(V (R 1)) \<mapsto> Bc True, (V (R 2)) \<mapsto> And (Geq (Num 100)) (Geq (Num 100))\<rbrakk>"
-  apply (simp add: t3_def)
+lemma medial_vend: "medial r1_r2_true (Guard vend) = \<lbrakk>(V (R 1)) \<mapsto> Bc True, (V (R 2)) \<mapsto> And (Geq (Num 100)) (Geq (Num 100))\<rbrakk>"
+  apply (simp add: vend_def)
   apply (rule ext)
   by simp
 
-lemma consistent_medial_t3: "consistent \<lbrakk>(V (R 1)) \<mapsto> Bc True, (V (R 2)) \<mapsto> And (Geq (Num 100)) (Geq (Num 100))\<rbrakk>"
+lemma consistent_medial_vend: "consistent \<lbrakk>(V (R 1)) \<mapsto> Bc True, (V (R 2)) \<mapsto> And (Geq (Num 100)) (Geq (Num 100))\<rbrakk>"
   apply (simp add: consistent_def)
   apply (rule_tac x="<R 1 := Num 0, R 2 := Num 100>" in exI)
   apply (simp del: Nat.One_nat_def)
   using consistent_empty_4 by auto
  
 (* We can do any number of "coin"s before doing a "vend" *)
-lemma "n > 0 \<longrightarrow> Contexts.can_take t3 (posterior_n n t2 (posterior empty t1))"
+lemma "n > 0 \<longrightarrow> Contexts.can_take vend (posterior_n n coin (posterior empty select))"
 proof (induct n)
 case 0
   then show ?case by simp
@@ -288,7 +288,7 @@ next
   case (Suc n)
   then show ?case
     apply (simp del: Nat.One_nat_def)
-    apply (simp only: t1_posterior posterior_t2_first posterior_n_t2_true_true Contexts.can_take_def)
-    by (simp only: medial_t3 consistent_medial_t3)
+    apply (simp only: select_posterior posterior_coin_first posterior_n_coin_true_true Contexts.can_take_def)
+    by (simp only: medial_vend consistent_medial_vend)
 qed
 end
