michael_formal/drinks_machine_change.thy
@@ -2,8 +2,8 @@ theory drinks_machine_change
   imports drinks_machine
 begin
 
-definition t3 :: "transition" where
-"t3 \<equiv> \<lparr>
+definition vend :: "transition" where
+"vend \<equiv> \<lparr>
         Label = ''vend'',
         Arity = 0,
         Guard = [(Ge (V (R 2)) (L (Num 100)))], (* This is syntactic sugar for ''Not (Lt (V (R 2)) (N 100))'' which could also appear *)
@@ -11,14 +11,14 @@ definition t3 :: "transition" where
         Updates = [(R 1, (V (R 1))), (R 2, (V (R 2)))]
       \<rparr>"
 
-definition vend :: "efsm" where
-"vend \<equiv> \<lparr> 
+definition drinks :: "efsm" where
+"drinks \<equiv> \<lparr> 
           S = [1,2,3],
           s0 = 1,
           T = \<lambda> (a,b) .
-              if (a,b) = (1,2) then [t1] (* If we want to go from state 1 to state 2 then t1 will do that *)
-              else if (a,b) = (2,2) then [t2] (* If we want to go from state 2 to state 2 then t2 will do that *)
-              else if (a,b) = (2,3) then [t3] (* If we want to go from state 2 to state 3 then t3 will do that *)
+              if (a,b) = (1,2) then [select] (* If we want to go from state 1 to state 2 then select will do that *)
+              else if (a,b) = (2,2) then [coin] (* If we want to go from state 2 to state 2 then coin will do that *)
+              else if (a,b) = (2,3) then [vend] (* If we want to go from state 2 to state 3 then drinks will do that *)
               else [] (* There are no other transitions *)
          \<rparr>"
 
@@ -27,35 +27,35 @@ definition vend :: "efsm" where
   They don't need to be translated to SAL
 *)
 
-lemmas transitions = t1_def t2_def t3_def
+lemmas transitions = select_def coin_def vend_def
 
-lemma "observe_trace vend (s0 vend) <> [] = []"
+lemma "observe_trace drinks (s0 drinks) <> [] = []"
   by simp
 
-lemma "observe_trace vend (s0 vend) <> [(''select'', [Str ''coke''])] = [[]]"
-  by (simp add: vend_def transitions step_def)
+lemma "observe_trace drinks (s0 drinks) <> [(''select'', [Str ''coke''])] = [[]]"
+  by (simp add: drinks_def transitions step_def)
 
-lemma "observe_trace vend (s0 vend) <> [(''select'', [Str ''coke'']), (''coin'', [Num 50])] = [[], [Num 50]]"
-  by (simp_all add: step_def vend_def transitions)
+lemma "observe_trace drinks (s0 drinks) <> [(''select'', [Str ''coke'']), (''coin'', [Num 50])] = [[], [Num 50]]"
+  by (simp_all add: step_def drinks_def transitions)
 
-lemma "observe_trace vend (s0 vend) <> [(''select'', [Str ''coke'']), (''coin'', [Num 50]), (''coin'', [Num 50])] = [[], [Num 50], [Num 100]]"
-  by (simp add: step_def vend_def transitions)
+lemma "observe_trace drinks (s0 drinks) <> [(''select'', [Str ''coke'']), (''coin'', [Num 50]), (''coin'', [Num 50])] = [[], [Num 50], [Num 100]]"
+  by (simp add: step_def drinks_def transitions)
 
-lemma "observe_trace vend (s0 vend) <> [(''select'', [Str ''coke'']), (''coin'', [Num 50]), (''coin'', [Num 50]), (''vend'', [])] = [[], [Num 50], [Num 100], [Str ''coke'', Num 0]]"
-  by (simp_all add: step_def vend_def transitions)
+lemma "observe_trace drinks (s0 drinks) <> [(''select'', [Str ''coke'']), (''coin'', [Num 50]), (''coin'', [Num 50]), (''vend'', [])] = [[], [Num 50], [Num 100], [Str ''coke'', Num 0]]"
+  by (simp_all add: step_def drinks_def transitions)
 
-lemma "observe_trace vend (s0 vend) <> [(''select'', [Str ''coke'']), (''coin'', [Num 50]), (''coin'', [Num 100]), (''vend'', [])] = [[], [Num 50], [Num 150], [Str ''coke'', Num 50]]"
-  by (simp_all add: step_def vend_def transitions)
+lemma "observe_trace drinks (s0 drinks) <> [(''select'', [Str ''coke'']), (''coin'', [Num 50]), (''coin'', [Num 100]), (''vend'', [])] = [[], [Num 50], [Num 150], [Str ''coke'', Num 50]]"
+  by (simp_all add: step_def drinks_def transitions)
 
 (*Stop when we hit a spurious input*)
-lemma "observe_trace vend (s0 vend) <> [(''select'', [Str ''coke'']), (''cat'', [Num 50])] = [[]]"
-  by (simp add: step_def vend_def transitions)
+lemma "observe_trace drinks (s0 drinks) <> [(''select'', [Str ''coke'']), (''cat'', [Num 50])] = [[]]"
+  by (simp add: step_def drinks_def transitions)
 
-lemma "\<not> (valid_trace (vend) [(''select'', [Str ''coke'']), (''cat'', [Num 50])])"
-  by(simp add: step_def vend_def transitions)
+lemma "\<not> (valid_trace (drinks) [(''select'', [Str ''coke'']), (''cat'', [Num 50])])"
+  by(simp add: step_def drinks_def transitions)
 
-lemma "observe_trace vend (s0 vend) <> [(''select'', [Str ''coke'']), (''cat'', [Num 50]), (''coin'', [Num 50])] = [[]]"
-  by (simp add: step_def vend_def transitions)
+lemma "observe_trace drinks (s0 drinks) <> [(''select'', [Str ''coke'']), (''cat'', [Num 50]), (''coin'', [Num 50])] = [[]]"
+  by (simp add: step_def drinks_def transitions)
 
 lemma "( t = []) \<Longrightarrow> (observe_trace e (s0 e) <> t = []) "
   by(simp)
